Unroll innermost loop in pack/unpack

frodo/code/Hacl.Impl.Frodo.Pack.fst
@@ -21,7 +21,7 @@ module S = Spec.Frodo.Pack
 #reset-options "--z3rlimit 50 --max_fuel 0 --max_ifuel 0 --using_facts_from '* -Spec'"
 
 private
-val shiftleft_bounds: d:size_nat{d <= 16} ->
+val shift_left_bounds: d:size_nat{d <= 16} ->
   Lemma (
     7 * d < bits U128 /\
     6 * d < bits U128 /\
@@ -31,22 +31,36 @@ val shiftleft_bounds: d:size_nat{d <= 16} ->
     2 * d < bits U128 /\
     1 * d < bits U128 /\
     0 * d < bits U128)
-let shiftleft_bounds d = ()
+let shift_left_bounds d = ()
+
+private
+let modifies_popped (#a:Type) (b1:buffer a) (b2:buffer a) (h0:mem) h1 (h2:mem) h3 :
+  Lemma
+    (requires
+      live h0 b1 /\
+      fresh_frame h0 h1 /\
+      modifies (loc_union (loc_buffer b1) (loc_buffer b2)) h1 h2 /\
+      get_tip h2 == get_tip h1 /\
+      popped h2 h3)
+    (ensures live h3 b1)
+  [SMTPat (fresh_frame h0 h1); SMTPat (popped h2 h3); SMTPat (live h0 b1);
+   SMTPat (modifies (loc_union (loc_buffer b1) (loc_buffer b2)) h1 h2)]
+= ()
+
 
 inline_for_extraction noextract
 val frodo_pack_inner:
     #n1:size_t
   -> #n2:size_t{v n1 * v n2 <= max_size_t /\ v n2 % 8 = 0}
   -> a:matrix_t n1 n2
-  -> d:size_t{v d * v n1 <= max_size_t /\ v n1 * (v n2 / 8) * v d <= max_size_t /\ v d <= 16}
-  -> res:lbytes (n1 *! (n2 /. size 8) *! d)
+  -> d:size_t{v d * v n1 <= max_size_t /\ v d * v n1 * v n2 <= max_size_t /\ v d <= 16}
+  -> res:lbytes (d *! n1 *! n2 /. size 8)
   -> i:size_t{v i < v n1}
   -> Stack unit
     (requires fun h -> live h a /\ live h res /\ disjoint a res)
-    (ensures  fun h0 _ h1 ->
-      live h1 res /\ modifies (loc_buffer res) h0 h1)
+    (ensures  fun h0 _ h1 -> live h1 res /\ modifies (loc_buffer res) h0 h1)
 let frodo_pack_inner #n1 #n2 a d res i =
-  shiftleft_bounds (v d);
+  shift_left_bounds (v d);
   push_frame();
   let maskd = to_u16 (u32 1 <<. size_to_uint32 d) -. u16 1 in
   let v16 = create #_ #16 (size 16) (u8 0) in
@@ -55,14 +69,14 @@ let frodo_pack_inner #n1 #n2 a d res i =
   let inv h1 (j:nat{j <= v n28}) =
     live h1 res /\
     live h1 v16 /\
-    modifies (loc_union (loc_buffer v16) (loc_buffer res)) h0 h1
+    modifies (loc_union (loc_buffer res) (loc_buffer v16)) h0 h1
   in
   let f (j:size_t{v j < v n28}) : Stack unit
     (requires fun h -> inv h (v j))
     (ensures  fun _ _ h2 -> inv h2 (v j + 1)) =
       Lemmas.lemma_matrix_index_repeati (v n1) (v n2) (v d) (v i) (v j);
       let start = (i *! n28 +! j) *! d in
-      assert_spinoff (v start + v d <= v n1 * (v n2 / 8) * v d);
+      assert_spinoff (v start + v d <= v d * v n1 * v n2 / 8);
       let aij0 = a.[i, size 8 *! j +! size 0] &. maskd in
       let aij1 = a.[i, size 8 *! j +! size 1] &. maskd in
       let aij2 = a.[i, size 8 *! j +! size 2] &. maskd in
@@ -93,19 +107,20 @@ val frodo_pack:
     #n1:size_t
   -> #n2:size_t{v n1 * v n2 <= max_size_t /\ v n2 % 8 = 0}
   -> a:matrix_t n1 n2
-  -> d:size_t{v d * v n1 <= max_size_t /\ v n1 * (v n2 / 8) * v d <= max_size_t /\ v d <= 16}
-  -> res:lbytes (n1 *! (n2 /. size 8) *! d)
+  -> d:size_t{v d * v n1 <= max_size_t /\ v d * v n1 * v n2 <= max_size_t /\ v d <= 16}
+  -> res:lbytes (d *! n1 *! n2 /. size 8)
   -> Stack unit
     (requires fun h -> live h a /\ live h res /\ disjoint a res)
     (ensures  fun h0 _ h1 ->
       live h1 res /\
       modifies (loc_buffer res) h0 h1 /\
       as_seq h1 res == S.frodo_pack (as_matrix h0 a) (v d))
+[@"c_inline"]
 let frodo_pack #n1 #n2 a d res =
   let h = ST.get () in
   push_frame();
   let h0 = ST.get () in
-  let inv h1 (j:nat{j <= v n1}) =
+  let inv h1 (i:nat{i <= v n1}) =
     live h1 res /\
     modifies (loc_buffer res) h0 h1
   in
@@ -113,6 +128,61 @@ let frodo_pack #n1 #n2 a d res =
   pop_frame();
   let h' = ST.get() in
   assume (as_seq h' res == S.frodo_pack (as_matrix h a) (v d))
+
+
+/// Unpack
+
+inline_for_extraction noextract
+val frodo_unpack_inner:
+    #n1:size_t
+  -> #n2:size_t{v n1 * v n2 <= max_size_t /\ v n2 % 8 = 0}
+  -> d:size_t{v d * v n1 <= max_size_t /\ v d * v n1 * v n2 <= max_size_t /\ v d <= 16}
+  -> b:lbytes (d *! n1 *! n2 /. size 8)
+  -> res:matrix_t n1 n2
+  -> i:size_t{v i < v n1}
+  -> Stack unit
+    (requires fun h -> live h b /\ live h res /\ disjoint b res)
+    (ensures  fun h0 _ h1 -> live h1 res /\ modifies (loc_buffer res) h0 h1)
+let frodo_unpack_inner #n1 #n2 d b res i =
+  shift_left_bounds (v d);
+  push_frame();
+  let maskd = to_u16 (u32 1 <<. size_to_uint32 d) -. u16 1 in
+  let v16 = create #_ #16 (size 16) (u8 0) in
+  let n28 = n2 /. size 8 in
+  let h0 = ST.get () in
+  let inv h1 (j:nat{j <= v n28}) =
+    live h1 res /\
+    live h1 v16 /\
+    modifies (loc_union (loc_buffer res) (loc_buffer v16)) h0 h1
+  in
+  let f (j:size_t{v j < v n28}) : Stack unit
+    (requires fun h -> inv h (v j))
+    (ensures  fun _ _ h2 -> inv h2 (v j + 1)) =
+      Lemmas.lemma_matrix_index_repeati (v n1) (v n2) (v d) (v i) (v j);
+      let start = (i *! n28 +! j) *! d in
+      assert_spinoff (v start + v d <= v d * v n1 * v n2 / 8);
+      let vij = sub b start d in
+      let src = update_sub v16 (size 16 -! d) d vij in
+      let templong = uint_from_bytes_be v16 in
+      res.[i, size 8 *! j +! size 0] <-
+        to_u16 (templong >>. size_to_uint32 (size 7 *! d)) &. maskd;
+      res.[i, size 8 *! j +! size 1] <-
+        to_u16 (templong >>. size_to_uint32 (size 6 *! d)) &. maskd;
+      res.[i, size 8 *! j +! size 2] <-
+        to_u16 (templong >>. size_to_uint32 (size 5 *! d)) &. maskd;
+      res.[i, size 8 *! j +! size 3] <-
+        to_u16 (templong >>. size_to_uint32 (size 4 *! d)) &. maskd;
+      res.[i, size 8 *! j +! size 4] <-
+        to_u16 (templong >>. size_to_uint32 (size 3 *! d)) &. maskd;
+      res.[i, size 8 *! j +! size 5] <-
+        to_u16 (templong >>. size_to_uint32 (size 2 *! d)) &. maskd;
+      res.[i, size 8 *! j +! size 6] <-
+        to_u16 (templong >>. size_to_uint32 (size 1 *! d)) &. maskd;
+      res.[i, size 8 *! j +! size 7] <-
+        to_u16 (templong >>. size_to_uint32 (size 0 *! d)) &. maskd
+  in
+  Lib.Loops.for (size 0) n28 inv f;
+  pop_frame()
 
 
 val frodo_unpack:
@@ -124,50 +194,17 @@ val frodo_unpack:
   -> Stack unit
     (requires fun h -> live h b /\ live h res /\ disjoint b res)
     (ensures  fun h0 _ h1 -> modifies (loc_buffer res) h0 h1 /\
-      as_seq h1 res == S.frodo_unpack (v n1) (v n2) (v d) (as_seq h0 b))
+      as_seq h1 res == S.frodo_unpack #(v n1) #(v n2) (v d) (as_seq h0 b))
 [@"c_inline"]
 let frodo_unpack n1 n2 d b res =
-  // TODO: This proof is fragile. It verifies in interactive mode but not from
-  // the command-line. FIX
-  admit();
-  assert (uint_v (size_to_uint32 d) < bits U32);
-  assert (uint_v (size_to_uint32 (size 7 *! d)) < bits U128);
+ let h = ST.get () in
   push_frame();
-  let maskd = (u32 1 <<. size_to_uint32 d) -. u32 1 in
-  let v16 = create (size 16) (u8 0) in
-  let n28 = n2 /. size 8 in
-  let bLen = d *! n1 *! n2 /. size 8 in
   let h0 = ST.get () in
-  let inv h1 j =
+  let inv h1 (i:nat{i <= v n1}) =
     live h1 res /\
-    live h1 v16 /\
-    modifies (loc_union (loc_buffer res) (loc_buffer v16)) h0 h1
+    modifies (loc_buffer res) h0 h1
   in
-  let f' (i:size_t{v i < v n1}): Stack unit
-      (requires fun h -> inv h (v i))
-      (ensures  fun _ _ h2 -> inv h2 (v i + 1)) =
-      let h0 = ST.get () in
-      let inv1 h1 j =
-        live h1 res /\
-        live h1 v16 /\
-        modifies (loc_union (loc_buffer res) (loc_buffer v16)) h0 h1
-      in
-      let f1 (j:size_t{0 <= v j /\ v j < v n28}): Stack unit
-        (requires fun h -> inv1 h (v j))
-        (ensures  fun _ _ h2 -> inv1 h2 (v j + 1)) =
-          assert (v i * v n2 < v n1 * v n2);
-          Lemmas.lemma_matrix_index_repeati (v n1) (v n2) (v d) (v i) (v j);
-          assert (v ((i *! n2 /. size 8 +! j) *! d) + v d <= v bLen);
-          let bij = sub #_ #(v bLen) #(v d) b ((i *! n2 /. size 8 +! j) *! d) d in
-          copy (sub #_ #_ #(v d) v16 (size 16 -! d) d) d bij;
-          let templong = uint_from_bytes_be #U128 v16 in
-          let h1 = ST.get () in
-          loop_nospec #h1 (size 8) res
-          (fun k ->
-            let resij = to_u32 (templong >>. size_to_uint32 (size 7 *! d -! d *! k)) &. maskd in
-            assert (8 * v j + v k < v n2);
-            mset res i (size 8 *! j +! k) (to_u16 resij)
-          ) in
-      Lib.Loops.for (size 0) n28 inv1 f1 in
-  Lib.Loops.for (size 0) n1 inv f';
-  pop_frame()
+  Lib.Loops.for (size 0) n1 inv (frodo_unpack_inner d b res);
+  pop_frame();
+  let h' = ST.get() in
+  assume (as_seq h' res == S.frodo_unpack #(v n1) #(v n2) (v d) (as_seq h' b))
